

- Consider penultimate layers of node.
- Expression for $\frac{\partial E_n(w)}{\partial a_1^{[2]}}$. Use $\delta_1^{[3]}$.

$$\delta_1^{[3]} \equiv \frac{\partial E_n(w)}{\partial a_1^{[3]}}$$

Chain rule:-

$$\frac{\partial E_n(w)}{\partial a_1^{[2]}} = \left[\frac{\partial E_n(w)}{\partial a_1^{[3]}} \right] \times \frac{\partial a_1^{[3]}}{\partial a_1^{[2]}}$$

\downarrow
 $\delta_1^{[3]}$

$$a_1^{[3]} = w_{11}^{[3]} h(a_1^{[2]}) + w_{12}^{[3]} h(a_2^{[2]}) + w_{13}^{[3]} h(a_3^{[2]})$$

$$\frac{\partial a_1^{[3]}}{\partial a_1^{[2]}} = w_{11}^{[3]} h'(a_1^{[2]})$$

$$\therefore \frac{\partial E_n(w)}{\partial a_1^{[2]}} = \delta_1^{[3]} w_{11}^{[3]} h'(a_1^{[2]}) \quad \text{--- (1)}$$

- Use this to calc $\frac{\partial E_n(w)}{\partial w_{11}^{[2]}}$

$$\frac{\partial E_n(w)}{\partial w_{11}^{[2]}} = \frac{\partial E_n(w)}{\partial a_1^{[2]}} \times \frac{\partial a_1^{[2]}}{\partial w_{11}^{[2]}} \quad \text{--- (2)}$$

$$a_1^{[2]} = w_{11}^{[2]} h(a_1^{[1]}) + w_{12}^{[2]} h(a_2^{[1]}) + w_{13}^{[2]} h(a_3^{[1]})$$

$$\frac{\partial a_1^{[2]}}{\partial w_{11}^{[2]}} = h(a_1^{[1]}) \quad \text{--- (3)}$$

① and ③ in ②

$$\frac{\partial E_n(w)}{\partial w_{11}^{[2]}} = \delta_1^{[3]} w_{11}^{[3]} h'(a_1^{[2]}) h(a_1^{[1]})$$

X ————— X